Playing around with binary search trees

teaching/taltech2018/sol/BinarySearchTree.fst
@@ -1,90 +1,121 @@
 module BinarySearchTree
 
-abstract type btree = 
+(* Binary trees *)
+
+private abstract type btree = 
   | Leaf : btree
   | Node : btree -> nat -> btree -> btree
 
-let rec exists_in (n:nat) (t:btree) : GTot bool =
+(* Search function / containment predicate for binary (search) trees *)
+
+private let rec btree_contains (t:btree) (n:nat) : GTot bool =
   match t with 
   | Leaf -> false
   | Node t1 m t2 -> 
       if n = m then true else 
-      if n < m then n `exists_in` t1 
-               else n `exists_in` t2
+      if n < m then t1 `btree_contains` n
+               else t2 `btree_contains` n
 
-let empty () : GTot btree = Leaf
+(* Empty binary tree *)
 
-let rec insert (t:btree) (n:nat) : GTot btree =
+private let empty_btree () : GTot btree = Leaf
+
+(* Insertion into a binary (search) tree *)
+
+private let rec btree_insert (t:btree) (n:nat) : GTot btree =
   match t with 
   | Leaf -> Node Leaf n Leaf
   | Node t1 m t2 -> 
       if n = m then Node t1 m t2 else
-      if n < m then Node (insert t1 n) m t2
-               else Node t1 m (insert t2 n)
+      if n < m then Node (btree_insert t1 n) m t2
+               else Node t1 m (btree_insert t2 n)
 
-let rec is_sorted_left (t:btree) (n:nat) : GTot bool = 
+(* Sortedness predicate for binary (search) trees *)
+
+private let rec sorted_left_of (t:btree) (n:nat) : GTot bool = 
   match t with
   | Leaf -> true
-  | Node t1 m t2 -> t1 `is_sorted_left` m && 
+  | Node t1 m t2 -> t1 `sorted_left_of` m && 
                     m < n && 
-                    t2 `is_sorted_right` m
+                    t2 `sorted_right_of` m
 
-and is_sorted_right (t:btree) (n:nat) : GTot bool = 
+and sorted_right_of (t:btree) (n:nat) : GTot bool = 
   match t with
   | Leaf -> true
-  | Node t1 m t2 -> t1 `is_sorted_left` m && 
+  | Node t1 m t2 -> t1 `sorted_left_of` m && 
                     m > n && 
-                    t2 `is_sorted_right` m
+                    t2 `sorted_right_of` m
 
-let rec is_sorted (t:btree) : GTot bool =
+private let rec sorted (t:btree) : GTot bool =
   match t with
   | Leaf -> true
-  | Node t1 n t2 -> t1 `is_sorted_left` n && t2 `is_sorted_right` n
+  | Node t1 n t2 -> t1 `sorted_left_of` n && 
+                    t2 `sorted_right_of` n
 
-abstract type stree = 
-  t:btree{is_sorted t}
+(* Useful lemmas about sortedness and the tree operations defined above *)
 
-let lemma_empty_is_sorted () : Lemma (is_sorted (empty ())) = 
-  ()
-
-let rec lemma_insert_is_sorted (t:stree) (n:nat) : Lemma (is_sorted (insert t n)) = 
+private let rec lemma_btree_insert_is_sorted (t:btree) (n:nat) : Lemma (requires (sorted t))
+                                                                       (ensures  (sorted (btree_insert t n))) = 
   match t with
   | Leaf -> ()
   | Node t1 m t2 -> 
       if n = m then () else
-      if n < m then lemma_insert_is_sorted t1 n
-               else lemma_insert_is_sorted t2 n
+      if n < m then lemma_btree_insert_is_sorted t1 n
+               else lemma_btree_insert_is_sorted t2 n
 
-let rec lemma_exists_insert_equal (t:stree) (n:nat) : Lemma (requires (n `exists_in` t))
-                                                            (ensures  (insert t n = t)) = 
+private let rec lemma_btree_insert_exists (t:btree) (n:nat) : Lemma (requires (sorted t))
+                                                                    (ensures  ((btree_insert t n) `btree_contains` n)) =
+  match t with
+  | Leaf -> ()
+  | Node t1 m t2 -> 
+      if n = m then () else
+      if n < m then lemma_btree_insert_exists t1 n
+               else lemma_btree_insert_exists t2 n
+
+private let rec lemma_exists_btree_insert_equal (t:btree) (n:nat) : Lemma (requires (sorted t && t `btree_contains` n))
+                                                                          (ensures  (btree_insert t n = t)) = 
   match t with
   | Node t1 m t2 -> 
       if n = m then () else 
-      if n < m then lemma_exists_insert_equal t1 n
-               else lemma_exists_insert_equal t2 n
+      if n < m then lemma_exists_btree_insert_equal t1 n
+               else lemma_exists_btree_insert_equal t2 n
 
-let rec lemma_insert_exists (t:stree) (n:nat) : Lemma (n `exists_in` (insert t n)) =
-  match t with
-  | Leaf -> ()
-  | Node t1 m t2 -> 
-      if n = m then () else
-      if n < m then lemma_insert_exists t1 n
-               else lemma_insert_exists t2 n
+(* Binary search trees = binary trees as defined above that are sorted *)
 
-(*
-let rec lemma_sorted_left_is_sorted (t:btree) (n:nat) : Lemma (requires (is_sorted_left t n))
-                                                              (ensures  (is_sorted t)) 
-                                                              [SMTPat (is_sorted_left t n)] =
-  match t with
-  | Leaf -> ()
-  | Node t1 m t2 -> lemma_sorted_left_is_sorted t1 m;                    
-                    lemma_sorted_right_is_sorted t2 m
+abstract type stree = 
+  t:btree{sorted t}
 
-and lemma_sorted_right_is_sorted (t:btree) (n:nat) : Lemma (requires (is_sorted_right t n))
-                                                           (ensures  (is_sorted t)) 
-                                                           [SMTPat (is_sorted_right t n)] =
-  match t with
-  | Leaf -> ()
-  | Node t1 m t2 -> lemma_sorted_left_is_sorted t1 m;
-                    lemma_sorted_right_is_sorted t2 m
-*)
+(* Binary search tree operations, derived from tree operations defined above*)
+
+let contains (t:stree) (n:nat) : GTot bool =
+  btree_contains t n
+
+let empty () : GTot stree = 
+  empty_btree ()
+
+let insert (t:stree) (n:nat) : GTot stree = 
+  lemma_btree_insert_is_sorted t n; 
+  btree_insert t n
+
+(* Sanity check lemmas *)
+
+private let lemma_contains_equals (t:stree) (n:nat) : Lemma (t `btree_contains` n = t `contains` n) = 
+  ()
+
+private let lemma empty_equals () : Lemma (empty_btree () = empty ()) = 
+  ()
+
+private let lemma_insert_equals (t:stree) (n:nat) : Lemma (btree_insert t n = insert t n) = 
+  ()
+  
+(* Important properties of binary search trees *)
+
+let rec lemma_insert_is_sorted (t:stree) (n:nat) : Lemma (sorted (btree_insert t n)) = 
+  lemma_btree_insert_is_sorted t n
+
+let rec lemma_insert_exists (t:stree) (n:nat) : Lemma ((btree_insert t n) `btree_contains` n) =
+  lemma_btree_insert_exists t n
+
+let rec lemma_exists_insert_equal (t:stree) (n:nat) : Lemma (requires (t `btree_contains` n))
+                                                            (ensures  (btree_insert t n = t)) = 
+  lemma_exists_btree_insert_equal t n
